---
layout: distill
title: UCB EECS 70 Discrete Mathematics and Probability Theory
categories: Notes
date: 2023-07-02
description: My answer for the UCB EECS 70 Discrete Mathematics and Probability Theory course.
tags:
  - Discrete Mathematics
  - Probability Theory
giscus_comments: true
related_posts: false

authors:
  - name: Pu Fanyi
    url: "https://pufanyi.github.io"
    affiliations:
      name: NTU, Singapore
      url: "https://www.ntu.edu.sg/"

toc:
  - name: Discussion 0A
  - name: Homework 0
  - name: Note 2
  - name: Note 3
  - name: Discussion 1A
  - name: Discussion 1B
  - name: Homework 1
---

Here is my answer for the [UCB EECS 70 Discrete Mathematics and Probability Theory](https://fa22.eecs70.org/) course.

Due to the absence of official answers, some of the answers to the questions may be incorrect, and we also welcome everyone to point them out.

---

## Discussion 0A

[Problem Link](https://fa22.eecs70.org/assets/pdf/dis00a.pdf)

### 1 Truth Tables

**(a)**

| $$P$$ | $$Q$$ | $$Q\lor P$$ | $$P\land(Q\lor P)$$ | $$P\land Q$$ |
| :---: | :---: | :---------: | :-----------------: | :----------: |
|   T   |   T   |      T      |          T          |      T       |
|   T   |   F   |      T      |          T          |      F       |
|   F   |   T   |      T      |          F          |      F       |
|   F   |   F   |      F      |          F          |      F       |

When $$P=\mathtt{T},Q=\mathtt{F}$$, $$\mathrm{LHS}=\mathtt{T}$$ but $$\mathrm{RHS}=\mathtt{F}$$.

So $$\mathrm{LHS}\not\equiv \mathrm{RHS}$$.

**(b)**

| $$P$$ | $$Q$$ | $$R$$ | $$P\lor Q$$ | $$(P\lor Q)\land R$$ | $$P\land R$$ | $$Q\land R$$ | $$(P\land R)\lor(Q\land R)$$ |
| :---: | :---: | :---: | :---------: | :------------------: | :----------: | :----------: | :--------------------------: |
| False | False | False |    False    |        False         |    False     |    False     |            False             |
| False | False | True  |    False    |        False         |    False     |    False     |            False             |
| False | True  | False |    True     |        False         |    False     |    False     |            False             |
| False | True  | True  |    True     |         True         |    False     |     True     |             True             |
| True  | False | False |    True     |        False         |    False     |    False     |            False             |
| True  | False | True  |    True     |         True         |     True     |    False     |             True             |
| True  | True  | False |    True     |        False         |    False     |    False     |            False             |
| True  | True  | True  |    True     |         True         |     True     |     True     |             True             |

So $$\mathrm{LHS}\equiv \mathrm{RHS}$$.

```python
from itertools import product

if __name__ == "__main__":
    tb = (False, True)
    for P, Q, R in product(tb, tb, tb):
        print('', P, Q, R, P or Q, (P or Q) and R,
              P and R, Q and R, (P and R) or (Q and R),
              '', sep='|')
```

**\(c\)**

| $$P$$ | $$Q$$ | $$R$$ | $$P\land Q$$ | $$(P\land Q)\lor R$$ | $$P\lor R$$ | $$Q\lor R$$ | $$(P\lor R)\land(Q\lor R)$$ |
| :---: | :---: | :---: | :----------: | :------------------: | :---------: | :---------: | :-------------------------: |
| False | False | False |    False     |        False         |    False    |    False    |            False            |
| False | False | True  |    False     |         True         |    True     |    True     |            True             |
| False | True  | False |    False     |        False         |    False    |    True     |            False            |
| False | True  | True  |    False     |         True         |    True     |    True     |            True             |
| True  | False | False |    False     |        False         |    True     |    False    |            False            |
| True  | False | True  |    False     |         True         |    True     |    True     |            True             |
| True  | True  | False |     True     |         True         |    True     |    True     |            True             |
| True  | True  | True  |     True     |         True         |    True     |    True     |            True             |

So $$\mathrm{LHS}\equiv \mathrm{RHS}$$.

```python
from itertools import product

if __name__ == "__main__":
    tb = (False, True)
    for P, Q, R in product(tb, tb, tb):
        print('', P, Q, R, P and Q, (P and Q) or R,
              P or R, Q or R, (P or R) and (Q or R),
              '', sep='|')
```

### 2 Propositional Practice

**(a)**

$$
\exists x\in\mathbb{R}, x\not\in\mathbb{Q}.
$$

**(b)**

$$
\forall n\in \mathbb{Z},\left((n\in\mathbb{N})\lor(n<0)\right)\land\lnot\left((n\in\mathbb{N})\land(n<0)\right).
$$

**\(c\)**

$$
\forall n\in \mathbb{N},\left(6\mid n\implies(2\mid n)\lor (3\mid n)\right).
$$

**(d)** All integers are rational numbers.

**(e)** All integers divisible by $$2$$ or $$3$$ are divisible by $$6$$.

**(f)** Any natural number greater than 7 can be decomposed into the sum of two natural numbers.

### 3 Converse and Contrapositive

**(a)**

$$
\forall n\in\mathbb{N}, (4\mid n\implies 2\mid n).
$$

It is true.

We let $$n=4k, k\in \mathbb{N}$$.

We have $$n=2\cdot (2k)$$, so $$2\mid n$$.

**(b)** If a natural number is not divisible by $$4$$, it is not divisible by $$2$$.

$$
\forall n\in\mathbb{N}, (4\nmid n\implies 2\nmid n).
$$

It is false.

A possible counterexample is when $$n=2$$, $$4\nmid 2$$, but $$2\mid 2$$.

**\(c\)** If a natural number is divisible by $$2$$, it is divisible by $$4$$.

$$
\forall n\in\mathbb{N}, (2\mid n\implies 4\mid n).
$$

It is false.

A possible counterexample is when $$n=2$$, $$2\mid 2$$, but $$4\nmid 2$$.

**(d)** If a natural number is divisible by $$2$$, it is divisible by $$4$$.

### 4 Equivalences with Quantifiers

**(a)**

$$
\begin{aligned}
\mathrm{LHS}&\equiv\forall x\ ((\exists y\ Q(x, y))\implies P(x))\\
&\equiv \forall x\ (\lnot(\exists y\ Q(x, y))\lor P(x))\\
&\equiv \forall x\ ((\forall y\ \lnot Q(x, y))\lor P(x))\\
&\equiv \forall x\forall y\ (\lnot Q(x, y)\lor P(x))\\
&\equiv \forall x\forall y\ (Q(x, y)\implies P(x))\\
&\not \equiv \forall x\exists y\ (Q(x, y)\implies P(x))\\
&\equiv \mathrm{RHS}
\end{aligned}
$$

To find one counterexample, we could let $$P(x)$$ to be contradictions, like "$$x$$ is an elephant", and $$Q(x, y)$$ be "$$x=y$$". On the one hand, for all $$x$$, $$\exists y\ Q(x, y)$$ is true because we could just let $$y=x$$, and $$P(x)$$ is false, so $$\mathrm{LHS}$$ is false. However, for all $$x$$, we just let $$y=x+1$$, then since $$Q(x, y)$$ is false, $$Q(x, y)\implies P(x)$$ is true, so $$\mathrm{RHS}$$ is true.

**(b)**

$$
\begin{aligned}
\mathrm{LHS}&\equiv\forall x\exists y\ \left(\lnot\left(P(x, y)\implies \lnot Q(x, y)\right)\right)\\
&\equiv\forall x\exists y\ \left(\lnot\left(\lnot P(x, y)\lor \lnot Q(x, y)\right)\right)\\
&\equiv\forall x\exists y\ \left(P(x, y)\land Q(x, y)\right)\\
&\not\equiv\forall x\left((\exists y\ P(x, y))\land (\exists y\ Q(x, y))\right)\\
&\equiv \mathrm{RHS}
\end{aligned}
$$

To find one counterexample, we could let $$P(x, y)$$ to be $$x=y$$, and $$Q(x, y)$$ be "$$x=y+1$$". On the one hand, when $$x=y$$, $$x\neq y+1$$, so $$P(x, y)\implies \lnot Q(x, y)$$ is true. So $$\mathrm{LHS}$$ is false. But for all $$x$$. For $$\exists y\ P(x, y)$$, we just let $$y=x$$, so it is true. And for $$\exists y\ Q(x, y)$$, we just let $$y = x - 1$$, so it is also true. In all $$\mathrm{RHS}$$ is true. So $$\mathrm{LHS}\not\equiv\mathrm{RHS}$$.

**\(c\)**

$$
\begin{aligned}
\mathrm{LHS}&\equiv \forall x\exists y\ (\lnot P(x)\lor Q(x,y))\\
\mathrm{RHS}&\equiv\forall x\ (\lnot P(x)\lor(\exists y\ Q(x, y)))
\end{aligned}
$$

If $$P(x)$$ is true, $$\mathrm{LHS}\equiv \forall x\exists y\ (\mathtt{F}\lor Q(x, y))\equiv \forall x\exists y\ Q(x, y)$$, $$\mathrm{RHS}\equiv\forall x\ (\mathtt{F}\lor (\exists y\ Q(x, y)))\equiv \forall x\exists y\ Q(x, y)$$. So $$\mathrm{LHS}\equiv \mathrm{RHS}$$.

If $$P(x)$$ is true, then $$\mathrm{LHS}\equiv \mathrm{RHS}\equiv \mathtt{T}$$.

In all $$\mathrm{LHS}\equiv\mathrm{RHS}$$.

---

## Homework 0

[Problem Link](https://fa22.eecs70.org/assets/pdf/hw00.pdf)

### 5 Propositional Practice

**(a)**

$$
\exists x\in\mathbb{R}\ ((x^2=0)\land(\forall y\in\mathbb{R}\ ((y^2=0)\implies (x=y)))).
$$

**(b)**

$$
\forall x\in\mathbb{Q}\ \forall y\in\mathbb{Q}\ \exists z\in \mathbb{Q}\ ((x=y)\lor (x<y<z)\lor(x>y>z)).
$$

**\(c\)**

$$
\forall x\in\mathbb{Z}\ ((x^2>4)\implies((x<-2)\lor(x>2))).
$$

**(d)** All real numbers are complex numbers.

**(e)** There is no integer solution of $$x^2-y^2=10$$.

**(f)** All greater than $$2$$ natural numbers can be decomposed into the sum of two prime numbers.

---

## Note 2

[Problem Link](https://fa22.eecs70.org/assets/pdf/notes/n2.pdf)

### 9 Exercises

**1\.**

$$
\begin{aligned}
n&\equiv\sum_{i=0}^{k-1}\left(a_i\cdot 10^i\right)\pmod 9\\
&\equiv \sum_{i=0}^{k-1}\left(a_i\cdot 10^i\mod 9\right)\pmod 9\\
&\equiv \sum_{i=0}^{k-1}\left(a_i\cdot\left(10^i\mod 9\right)\right)\pmod 9\\
&\equiv \sum_{i=0}^{k-1}\left(a_i\cdot\left(10\mod 9\right)^i\right)\pmod 9\\
&\equiv \sum_{i=0}^{k-1}a_i\pmod 9
\end{aligned}
$$

**2\.**

$$
\begin{aligned}
&\text{$a^2$ is even}\implies \text{$a$ is even}\\
\equiv&\lnot(\text{$a$ is even})\implies \lnot(\text{$a^2$ is even})\\
\equiv&\text{$a$ is odd}\implies \text{$a^2$ is odd}
\end{aligned}
$$

Let $$a=2k+1, k\in \mathbb{Z}$$, we have $$a^2=4k^2+4k+1=2(2k^2+1)+1$$, so $$a^2$$ is odd.

So $$a\text{ is odd}\implies a^2\text{ is odd}$$ holds, so Lemma 2.2 holds.

---

## Note 3

[Problem Link](https://fa22.eecs70.org/assets/pdf/notes/n3.pdf)

**1\.** We proceed by induction on $$n$$.

_Base Case:_ When $$n=1$$, $$\mathrm{LHS}=\mathrm{RHS}=1$$. So base case Holds.

_Induction Hypothesis:_ Assume that $$\sum_{i=1}^{k} i = \frac{1}{6}k(k+1)(2k+1)$$.

_Induction Step:_ When $$n=k+1$$,

$$
\begin{aligned}
\sum_{i=1}^{k+1}i&=(k+1)+\sum_{i=1}^{k} i\\
&=\frac{1}{6}k(k+1)(2k+1)+k+1\\
&=\frac{1}{6}(k+1)(2k^2+k+6k+6)\\
&=\frac{1}{6}(k+1)(2k^2+7k+6)\\
&=\frac{1}{6}(k+1)(k+2)(2k+3)
\end{aligned}
$$

Thus, $$\forall n\in\mathbb{N}$$, $$\sum_{i=1}^{n} i = \frac{1}{6}n(n+1)(2n+1)$$ holds.

**2\.** We proceed by induction on $$n$$.

_Base Case:_ When $$n=1$$, $$\mathrm{LHS}=\mathrm{RHS}=1+x$$. So base case Holds.

_Induction Hypothesis:_ Assume that $$(1+x)^k\ge 1+kx$$, for $$k\in \mathbb{N}$$.

_Induction Step:_ When $$n=k+1$$,

$$
\begin{aligned}
(1+x)^{k+1}&=(1+x)\cdot(1+x)^k\\
&\ge(1+x)\cdot(1+kx)\\
&=1+(k+1)\cdot x+kx^2\\
&\ge 1+(k+1)\cdot x
\end{aligned}
$$

Thus, $$\forall n\in\mathbb{N}, x>-1, \ (1+x)^n\ge 1+nx$$ holds.

**3\.** We proceed by induction on $$n$$.

_Base Case:_ When $$n=2$$, $$\mathrm{LHS}=2<4=\mathrm{RHS}$$. So base case Holds.

_Induction Hypothesis:_ Assume that $$k!<k^k$$, for $$k\in \mathbb{N}, k>1$$.

_Induction Step:_ When $$n=k+1$$,

$$
\begin{aligned}
(k+1)!&=(k+1)\cdot k!\\
&<(k+1)\cdot k^k\\
&<(k+1)\cdot (k+1)^k\\
&=(k+1)^{k+1}
\end{aligned}
$$

Thus, $$\forall n\in\mathbb{N}, n>1, \ n!<n^n$$ holds.

**4\.** We define an ask $$A\to B$$ means asking A if he know B. And we define $$f(n)$$ be the times of asking.

_Base Case:_ When $$n=2$$, there are just two people A and B. We could ask $$A\to B$$ and $$B\to A$$. And now we know everything and it is easy for us to find the answer. We asked $$3n-4=2$$ times. So $$f(n)\le 3n-4$$ holds for $$n=1$$.

_Induction Hypothesis:_ Assume that if there are $$k$$ people, we could use $$3k-4$$ asks to find the answer.

_Induction Step:_ When $$n=k+1$$, we could randomly choose two people A and B, asking $$A\to B$$.

Now there are two cases:

1. If A don't know B. Then we could know that B is not celebrity. So we could just firstly remove B and solve the remaining $$k$$ people to find the "celebrity" for these $$k$$ people, which is C. (If now found, just return "not found".) And after that, we should check if B knows C and C doesn't know B. It cost $$f(k + 1)=3+f(k)\le 3+(3k-4)=3(k+1)-4$$.
2. If A knows B. Then we could know that A is not celebrity. Then we can prove as in the first case, changing B to A.

So $$f(k+1)\le 3(k+1)-4$$. And as a conclusion, $$f(n)\le 3n-4$$ holds for all $$n\in\mathbb{N}, n\ge 2$$.

**5\.** The python code shows below:

```python
def solve(n):
    base_case = [(3, 0), (2, 1), (1, 2), (0, 3)]
    return base_case[n % 4][0] + (n - 12) // 4, base_case[n % 4][1]
```

The largest number of 5c stamps my algorithm will ever use is $$3$$.

---

## Discussion 1A

[Problem Link](https://fa22.eecs70.org/assets/pdf/dis01a.pdf)

### 1 Contraposition

$$
\begin{aligned}
  &(a + b < c + d)\implies (a < c)\lor(b < d)\\
  \equiv & \lnot((a < c)\lor(b < d))\implies \lnot(a+b < c+d)\\
  \equiv & (a\ge c)\land(b\ge d) \implies (a+b\ge c+d)
\end{aligned}
$$

### 2 Numbers of Friends

We let the $$i$$-th person have $$a_i$$ friends. We have $$a_i\in[0, n-1]\cap \mathbb{Z}$$.

Then we check if there exist $$k\in [0, n-1]\cap\mathbb{Z}$$, $$\forall i, a_i\neq k$$.

1. $$\exists k\in [0, n-1]\cap\mathbb{Z}, \forall i, a_i\neq k$$. Which means, $$\forall i, a_i\in [0, n-1]\cap\mathbb{Z}\backslash\{k\}$$. And since $$\left\|[0, n-1]\cap\mathbb{Z}\backslash\{k\}\right\|=n-1$$, and there are $$n$$ numbers. Due to the Pigeonhole Principle, there must be $$2$$ of them have the same number.
2. If $$\forall k\in [0, n-1]\cap\mathbb{Z}, \exists i, a_i=k$$, there must be some one with $$0$$ friends (name A) and some one with $$n-1$$ friends (name B). A have $$0$$ friends shows that A and B are not friends, but B have $$n-1$$ friends shows that A and B are friends. This forms a contradiction, so this case is impossible.

In all, there must be at least $$2$$ of them have the same number of friends at the party.

### 3 Pebbles

If there is no all-red column exist, which means all column has a blue pebble, for every column, we could just choose that blue pebble, then there exist a way choosing makes no red pebble. So there must exist all-red column.

### 4 Preserving Set Operations

**(a)** We want to prove $$f^{-1}(A\cup B)\subseteq f^{-1}(A)\cup f^{-1}(B)$$ and $$f^{-1}(A\cup B)\supseteq f^{-1}(A)\cup f^{-1}(B)$$.

We first show $$f^{-1}(A\cup B)\subseteq f^{-1}(A)\cup f^{-1}(B)$$.

Let $$x\in f^{-1}(A\cup B)$$, which means $$f(x)\in A\cup B$$. So $$(f(x)\in A)\lor (f(x)\in B)$$. So $$\left(x\in f^{-1}(A)\right)\lor \left(x\in f^{-1}(B)\right)$$, which means $$x\in f^{-1}(A)\cup f^{-1}(B)$$. So $$f^{-1}(A\cup B)\subseteq f^{-1}(A)\cup f^{-1}(B)$$.

Then let's prove $$f^{-1}(A\cup B)\supseteq f^{-1}(A)\cup f^{-1}(B)$$.

We let $$x\in f^{-1}(A)\cup f^{-1}(B)$$, which means $$x\in f^{-1}(A)$$ or $$x\in f^{-1}(B)$$. So $$f(x)\in A$$ or $$f(x)\in B$$, which is $$f(x)\in A\cup B$$. So $$x\in f^{-1}(A\cup B)$$. So $$f^{-1}(A)\cup f^{-1}(B)\subseteq f^{-1}(A\cup B)$$.

In all, $$f^{-1}(A\cup B)=f^{-1}(A)\cup f^{-1}(B)$$.

**(b)** We want to prove $$f(A\cup B)\subseteq f(A)\cup f(B)$$ and $$f(A\cup B)\supseteq f(A)\cup f(B)$$.

We firstly prove $$f(A\cup B)\subseteq f(A)\cup f(B)$$. Let $$x\in f(A\cup B)$$, which is $$\exists y\in A\cup B, f(y)=x$$. So $$\exists y\in A, f(y)=x$$ or $$\exists y\in B, f(y)=x$$. So $$x\in f(A)$$ or $$x\in f(B)$$. So $$x\in f(A)\cup f(B)$$. So $$f(A\cup B)\subseteq f(A)\cup f(B)$$.

Then we want to prove $$f(A\cup B)\supseteq f(A)\cup f(B)$$. Let $$x\in f(A)\cup f(B)$$, which is $$x\in f(A)$$ or $$x\in f(B)$$. So $$\exists y\in A, x=f(y)$$ or $$\exists y\in B, x = f(y)$$. So $$\exists y\in A\cup B, x = f(y)$$. So $$x\in f(A\cup B)$$. So $$f(A)\cup f(B)\subseteq f(A\cup B)$$.

In all $$f(A\cup B)=f(A)\cup f(B)$$.

---

## Discussion 1B

[Problem Link](https://fa22.eecs70.org/assets/pdf/dis01b.pdf)

### 1 Natural Induction on Inequality

_The same as Note 3 Question 2._

We proceed by induction on $$n$$.

_Base Case:_ When $$n=1$$, $$\mathrm{LHS}=\mathrm{RHS}=1+x$$. So base case Holds.

_Induction Hypothesis:_ Assume that $$(1+x)^k\ge 1+kx$$, for $$k\in \mathbb{N}$$.

_Induction Step:_ When $$n=k+1$$,

$$
\begin{aligned}
(1+x)^{k+1}&=(1+x)\cdot(1+x)^k\\
&\ge(1+x)\cdot(1+kx)\\
&=1+(k+1)\cdot x+kx^2\\
&\ge 1+(k+1)\cdot x
\end{aligned}
$$

Thus, $$\forall n\in\mathbb{N}, x>0, \ (1+x)^n\ge 1+nx$$ holds.

### 2 Make It Stronger

**(a)** No. If we let $$a_n\le 3^{2^n}$$, $$a_{n+1}=3a_n^2\le 3\cdot\left(3^{2^n}\right)^2=3^{2^{n+1}+1}$$. But $$3^{2^{n+1}+1}\ge 3^{2^{n+1}}$$, so it doesn't work.

**(b)** Let's prove by induction.

_Base Case:_ When $$n=1$$, $$a_1=1$$, $$3^{2^n-1}=3$$. So $$a_n\le 3^{2^n-1}$$ holds for $$n=1$$.

_Induction Hypothesis:_ Assume that $$a_k\le 3^{2^k-1}$$, for $$k\in \mathbb{N}$$.

_Induction Step:_ When $$n=k+1$$:

$$
a_{k+1}=3a_{k}^2\le 3\cdot \left(3^{2^k-1}\right)^2=3^{2^{k+1}-1}.
$$

So for all $$n\in\mathbb{N}^+$$, $$a_n\le 3^{2^n-1}$$.

**\(c\)** For $$n\in\mathbb{N}$$, $$a_n\le 3^{2^n-1}=\frac{1}{3}\cdot 3^{2^n}\le 3^{2^n}$$.

### 3 Binary Numbers

We proceed by induction on $$n$$.

_Base Case:_ When $$n=1$$, let $$c_0=1$$, $$n=1\cdot 2^0$$. So the assumption holds when $$n=1$$.

_Induction Hypothesis:_ We assume that the proposition holds for $$n\le t$$.

_Induction Step:_ We use the parity of t+1 for discussion.

If $$t + 1$$ is an odd number. Let $$\frac{t}{2}=\sum_{i=0}^k c_k\cdot 2^k$$, then $$t + 1=2\cdot \frac{t}{2}+1=2\sum_{i=0}^k c_i\cdot 2^i+1=\sum_{i=1}^{k+1}c_{i-1}\cdot 2^i+1\cdot 2^0$$.

If $$t+1$$ is an even number. Let $$\frac{t + 1}{2}=\sum_{i=0}^k c_i\cdot 2^i$$, then $$t+1=2\cdot\frac{t+1}{2}=2\sum_{i=0}^k c_i\cdot 2^i=\sum_{i=1}^{k+1} c_i\cdot 2^i+0\cdot 2^0$$.

In all, the proposition holds.

### 4 Fibonacci for Home

Let $$P(n)$$ be the proposition that $$2\mid F_{3n}$$. Let's prove it by induction.

_Base Case:_ When $$n=1$$, $$F_{3n}=2$$ so $$2\mid F_{3n}$$.

_Induction Hypothesis:_ We assume that $$2\mid F_{3k}$$ when $$k\in\mathbb{N}$$.

_Induction Step:_

$$
\begin{aligned}
F_{3(k+1)}&\equiv F_{3k+3}\pmod 2\\
&\equiv F_{3k+2}+F_{3k+1}\pmod 2\\
&\equiv F_{3k+1}+F_{3k}+F_{3k+1}\pmod 2\\
&\equiv 2F_{3k+1}+F_{3k}\pmod 2\\
&\equiv 0\pmod 2
\end{aligned}
$$

So $$2\mid F_{3(k+1)}$$.

In all, $$\forall n\in \mathbb{N}, 2\mid F_{3n}$$.

---

## Homework 1

[Problem Link](https://fa22.eecs70.org/assets/pdf/hw01.pdf)

### 1 Solving a System of Equations

Let the prices for an apple, for a beet, and for a carrot be $$a, b, c$$ separately. Then we have:

$$
\begin{bmatrix}
    1   &   1   &   1   \\
    2   &   3   &   0   \\
    1   &   2   &   3
\end{bmatrix}
\cdot
\begin{bmatrix}
    a\\
    b\\
    c
\end{bmatrix}
=
\begin{bmatrix}
16\\
23\\
35
\end{bmatrix}
$$

```Matlab
A = [1 1 1; 2 3 0; 1 2 3];
b = [16; 23; 35];
x = inv(A) * b;
disp(x);
```

Solving this equation, we get $$x=\begin{bmatrix}4&5&7\end{bmatrix}^{\mathrm{T}}$$. So $$a=4, b=5, c=7$$.

### 2 Calculus Review

**(a)**

$$
\begin{aligned}
\int_{0}^{\infty}e^{-t}\sin t\ \mathrm{d}t&=-\int_{0}^{\infty}\sin t\ \mathrm{d}\left(e^{-t}\right)\\
&=-\left(\left(\sin(t)\cdot e^{-t}\right)_0^{\infty}-\int_{0}^\infty e^{-t}\ \mathrm{d}(\sin t)\right)\\
&=\int_{0}^{\infty}e^{-t}\cos t\ \mathrm{d}t\\
&=-\int_{0}^{\infty}\cos t\ \mathrm{d}\left(e^{-t}\right)\\
&=-\left(\left(e^{-t}\cos t\right)_{0}^{\infty}-\int_{0}^{\infty}e^{-t}\ \mathrm{d}(\cos t)\right)\\
&=\int_{0}^{\infty}e^{-t}\ \mathrm{d}(\cos t)-\left(e^{-t}\cos t\right)_{0}^{\infty}\\
&=-\int^\infty_0e^{-t}\sin t\ \mathrm{d}t+1
\end{aligned}
$$

So,

$$
\int_{0}^{\infty}e^{-t}\sin t\ \mathrm{d}t=-\int_{0}^{\infty}e^{-t}\sin t\ \mathrm{d}t+1.
$$

Which is

$$
\int_{0}^{\infty}e^{-t}\sin t\ \mathrm{d}t=\frac{1}{2}.
$$

```Matlab
syms x;
disp(int(sin(x) * exp(-x), 0, inf));
```

**(b)**

$$
f'(x)=2x\cdot e^{-x^4}
$$

Since $$e^{-x^4}>0$$, $$f'(x)<0$$ when $$x<0$$ and $$f'(x)>0$$ when $$x>0$$.

So when $$x=0$$, the minimum value of $$f(x)$$ is $$0$$.

**\(c\)**

$$
\begin{aligned}
\iint_R 2x+y\ \mathrm{d}A&=\int_0^1\mathrm{d}x\int_{0}^{x}2x+y\ \mathrm{d}y\\
&=\int_{0}^{1}\left(2xy+\frac{1}{2}y^2\right)_{y=0}^{y=x}\mathrm{d}x\\
&=\int_{0}^{1}\frac{5}{2}x^2\ \mathrm{d}x\\
&=\frac{5}{6}
\end{aligned}
$$

### 3 Implication

**(a)** True.

**(b)** False. Let $$Q(x, y)$$ be $$x=y$$.

**\(c\)** True. For all $$y$$, we just choose the $$x$$ previously selected.

**(d)** True.

### 4 Logical Equivalence?

**(a)** True.

$$
\begin{aligned}
\forall x\ (P(x)\land Q(x))&\equiv\bigwedge_{x}(P(x)\land Q(x))\\&\equiv\left(\bigwedge_x P(x)\right)\land\left(\bigwedge_x Q(x)\right)\\
&\equiv \left(\forall x\ P(x)\right)\land\left(\forall x\ Q(x)\right)
\end{aligned}
$$

**(b)** False.

Let $$P(x)=(x>0), Q(x)=(x\le 0)$$. $$\forall x\ (P(x)\land Q(x))$$ is true but $$\left(\forall x\ P(x)\right)\lor\left(\forall x\ Q(x)\right)$$ is false.

**\(c\)** True.

$$
\begin{aligned}
\exists x\ (P(x)\lor Q(x))&\equiv\bigvee_{x}(P(x)\lor Q(x))\\&\equiv\left(\bigvee_x P(x)\right)\lor\left(\bigvee_x Q(x)\right)\\
&\equiv \left(\exists x\ P(x)\right)\lor\left(\exists x\ Q(x)\right)
\end{aligned}
$$

**(d)** False.

Let $$P(x)=(x=2)$$ and $$Q(x)=(x=3)$$. $$\mathrm{LHS}$$ is false but $$\mathrm{RHS}$$ is true.

### 5 Preserving Set Operations

**(a)**

$$
\begin{aligned}
&x\in f^{-1}(A\cap B)\\
\Longleftrightarrow\ &f(x)\in A\cap B\\
\Longleftrightarrow\ &\left(f(x)\in A\right)\land \left(f(x)\in B\right)\\
\Longleftrightarrow\ &\left(x\in f^{-1}(A)\right)\land \left(x\in f^{-1}(B)\right)\\
\Longleftrightarrow\ &x\in f^{-1}(A)\cap f^{-1}(B)
\end{aligned}
$$

So $$f^{-1}(A\cap B)=f^{-1}(A)\cap f^{-1}(B)$$.

**(b)**

$$
\begin{aligned}
&x\in f^{-1}(A\setminus B)\\
\Longleftrightarrow\ &f(x)\in A\setminus B\\
\Longleftrightarrow\ &(f(x)\in A)\land (f(x)\not\in B)\\
\Longleftrightarrow\ &(x\in f^{-1}(A))\land (x\not\in f^{-1}(B))\\
\Longleftrightarrow\ &x\in f^{-1}(A)\setminus f^{-1}(B)
\end{aligned}
$$

So $$f^{-1}(A\setminus B)=f^{-1}(A)\setminus f^{-1}(B)$$.

**\(c\)**

$$
\begin{aligned}
&y\in f(A\cap B)\\
\Longleftrightarrow\ &\exists x\in A\cap B, f(x)=y\\
\implies&(\exists x \in A, f(x)=y)\land (\exists x\in B, f(x)=y)\\
\Longleftrightarrow\ &(y\in f(A))\land (y\in f(B))\\
\Longleftrightarrow\ &y\in f(A)\cap f(B)
\end{aligned}
$$

So $$f(A\cap B)\subseteq f(A)\cap f(B)$$.

The counterexample for $$f(A\cap B)= f(A)\cap f(B)$$ is when $$A=\{2\}$$ and $$B = \{-2\}$$, and we let $$f(x)=x^2$$. $$f(A\cap B)=\emptyset$$ but $$f(A)\cap f(B)=\{4\}$$.

**(d)**

$$
\begin{aligned}
&y\in f(A\setminus B)\\
\Longleftrightarrow\ &\exists x\in A\setminus B, f(x)=y\\
\impliedby\ &(\exists x \in A, f(x)=y)\land (\forall x\in B, f(x)\neq y)\\
\Longleftrightarrow\ &(y\in f(A))\land (y\not\in f(B))\\
\Longleftrightarrow\ &y\in f(A)\setminus f(B)
\end{aligned}
$$

So $$f(A\setminus B)\supseteq f(A)\setminus f(B)$$.

The counterexample for $$f(A\setminus B)= f(A)\setminus f(B)$$ is when $$A=\{-2, 2\}$$ and $$B = \{-2\}$$, and we let $$f(x)=x^2$$. $$f(A\setminus B)=\{4\}$$ but $$f(A)\cap f(B)=\emptyset$$.

### 6 Prove or Disprove

**(a)** True. Let $$n=2k+1$$, $$k\in \mathbb{Z}$$. $$n^2+4n=4k^2+12k+5$$ is an odd number.

**(b)** True.

$$
\begin{aligned}
&a + b\le 15\implies (a\le 11) \lor (b\le 4)\\
\equiv\ &\lnot((a\le 11) \lor (b\le 4))\implies \lnot(a + b\le 15)\\
\equiv\ &(a > 15)\land (b>4)\implies a + b > 15
\end{aligned}
$$

**\(c\)** True.

$$
\begin{aligned}
&r^2\not\in \mathbb{Q}\implies r
\not\in \mathbb{Q}\\
\equiv\ &\lnot(r
\not\in \mathbb{Q})\implies \lnot(r^2\not\in \mathbb{Q})\\
\equiv\ &r
\in \mathbb{Q}\implies r^2\in \mathbb{Q}
\end{aligned}
$$

Let $$r=\frac{p}{q}$$, where $$p, q\in \mathbb{Z}$$ and $$\gcd(p, q) = 1$$. $$r^2=\frac{p^2}{q^2}\in\mathbb{Q}$$.

**(d)** False.

```python
from math import factorial

if __name__ == "__main__":
    n = 10
    print(5 * n ** 3 > factorial(n))
```

### 7 Rationals and Irrationals

We use proof by contradiction. Let $$x\in \mathbb{Q}, y\in\mathbb{R}\setminus\mathbb{Q}, z\in\mathbb{Q}$$ and $$z=xy$$.

But $$y = \frac{z}{x}\in \mathbb{Q}$$, which conflicts with $$y\in \mathbb{R}\setminus\mathbb{Q}$$, so $$z$$ must be irrational.

### 8 Twin Primes

**(a)** If $$3\mid p$$, $$p$$ is not a prime number. So $$3\nmid p$$. So $$p\equiv 1\pmod 3$$ or $$p\equiv 2\equiv -1\pmod 3$$.

So $$p$$ is of the form $$3k + 1$$ or $$3k - 1$$ for some integer $$k$$.

**(b)** If the three prime numbers are $$p, p + 2, p + 4\ (p>3)$$, we could let $$p=3k\pm 1$$.

If $$p=3k + 1$$, we have $$p + 2=3k + 3 = 3(k + 1)$$ is not a prime number.

If $$p=3k - 1$$, we have $$p + 4 = 3k + 3 = 3(k + 1)$$.

So $$5$$ is the only prime number that takes part in two different twin prime pairs.
